first draft of the Imp --> Vellvm compiler

src/coq/Compiler.v
@@ -1,10 +1,49 @@
-Require Import ZArith String Omega Lists Equalities MSets.
+Require Import ZArith String Omega List Equalities MSets.
 
 (* Vellvm dependencies *)
 Require Import Vellvm.Classes Vellvm.Ollvm_ast Vellvm.AstLib.
 
 (* Logical Foundations dependencies *)
 Require Import Imp Maps.
+
+(* "Flattened" representation of Vellvm code *)
+Inductive elt :=
+| L (lbl:block_id)
+| I (id:instr_id) (ins:instr)
+| T (id:instr_id) (t:terminator)
+.    
+
+Fixpoint monad_fold_left {A B} `{Monad M} (f : A -> B -> M A) (l:list B) (a:A) : M A :=
+  match l with
+  | [] => mret a
+  | x::xs =>
+    'y <- monad_fold_left f xs a;
+      f y x
+  end.
+
+Definition blocks_of_elts (entry_label:block_id) (code:list elt) : option (list block) :=
+  '(insns, term_opt, blks) <-
+   monad_fold_left
+   (fun '(insns, term_opt, blks) e =>
+      match e with
+      | L l =>
+        match term_opt with
+        | None => 
+          if (List.length insns) == 0 then mret ([], None, blks)
+          else None
+        | Some (id, t) =>
+          mret ([], None, (mk_block l insns t id)::blks)
+        end
+      | T id t  => mret ([], Some (id, t), blks)
+      | I uid insn => mret ((uid,insn)::insns, term_opt, blks)
+      end
+   ) code ([], None, []) 
+  ;
+    match term_opt with
+    | None => None
+    | Some (id, t) =>
+      mret ((mk_block entry_label insns t id) :: blks)
+    end.
 
 
 (* Auxilliary definitions for working with Identifiers ---------------------- *)
@@ -61,30 +100,191 @@ Instance FV_com : FV com := fv_com.
 
 (* LLVM Identifier generation monad ----------------------------------------- *)
 
-Definition GenSym A := ST int A.
-Definition gensym : () -> GenSym (local_id) :=
-  fun _ => fun n => (1+n, Anon (n))%Z.
+Definition GenSym A := ST (int*int) (option A).
 
+Definition gensym_map (A B:Type) (f:A->B) (g:GenSym A) : GenSym B :=
+  fun s =>
+    let '(n, x) := g s in
+    match x with
+    | None => (n, None)
+    | Some a => (n, Some (f a))
+    end.
+
+Instance gensym_functor : @Functor GenSym := gensym_map.
+
+Definition gensym_ret (A:Type) (x:A) : GenSym A :=
+  fun s => (s, Some x).
+
+Definition gensym_bind (A B:Type) (g:GenSym A) (f:A -> GenSym B) : GenSym B :=
+  fun s =>
+    let '(n, x) := g s in
+    match x with
+    | None => (n, None)
+    | Some a => (f a) n
+    end.
+Program Instance gensym_monad : (@Monad GenSym) gensym_functor := _.
+Next Obligation.
+  split.
+  - exact gensym_ret.
+  - exact gensym_bind.
+Defined.    
+
+Definition run {A} (g : GenSym A) : option A :=
+  let '(_, x) := g (0,0)%Z in x.
+
+Definition lift {A} (m:option A) : GenSym A :=
+  fun s => (s, m).
+
+Definition gensym : () -> GenSym (local_id) :=
+  fun _ => fun '(n,m) => ((1+n,m), Some (Anon (n)))%Z.
+
+Definition genvoid : () -> GenSym (instr_id) :=
+  fun _ => fun '(n,m) => ((n,1+m), Some (IVoid m))%Z.
 
 (* A context maps Imp variables to Vellvm identifiers
    Invariant: 
       storage space for an Imp variable is represented as an alloca'ed 
       ctxt (Id X) is the identifier for the pointer to the storage for X.
-
 *)
 Definition ctxt := partial_map ident.
 
-Inductive elt :=
-| L (lbl:block_id)
-| I (id:instr_id) (ins:instr)
-| T (id:instr_id) (t:terminator)
-.    
+Definition val_of_nat (n:nat) : value :=
+  SV (VALUE_Integer (Z.of_nat n)).
+
+Definition val_of_ident (id:ident) : value :=
+  SV (VALUE_Ident id).
+
+Definition val_of_bool (b:bool) : value :=
+  SV (VALUE_Bool b).
+
+Definition i1 := TYPE_I (1)%Z.
+Definition i64 := TYPE_I (64)%Z.
+Definition i64ptr := TYPE_Pointer i64.
+
+(* Note: list of instructions in code is generated in reverse order *)
+Fixpoint compile_aexp (g:ctxt) (a:aexp) : GenSym (value * list elt) :=
+  let compile_binop (op:ibinop) (a1 a2:aexp) :=
+      '(v1, code1) <- compile_aexp g a1;
+      '(v2, code2) <- compile_aexp g a2;
+      'lid <- gensym ();
+      mret (val_of_ident (ID_Local lid), [I (IId lid) (INSTR_Op (SV (OP_IBinop op i64 v1 v2)))] ++ code2 ++ code1)
+  in
+  match a with
+  | ANum n => mret (val_of_nat n, [])
+
+  | AId x =>
+    'uid <- lift (g x);
+    'lid <- gensym ();
+     mret (val_of_ident (ID_Local lid), [I (IId lid) (INSTR_Load false i64 (i64ptr, val_of_ident uid) None)])
+
+  | APlus a1 a2 => compile_binop (Add false false) a1 a2
+  | AMinus a1 a2 => compile_binop (Sub false false) a1 a2
+  | AMult a1 a2 => compile_binop (Mul false false) a1 a2
+  end.
+
+    
+Fixpoint compile_bexp (g:ctxt) (b:bexp) : GenSym (value * list elt) :=
+  let compile_icmp (cmp:icmp) (a1 a2:aexp) :=
+      '(v1, code1) <- compile_aexp g a1;
+      '(v2, code2) <- compile_aexp g a2;
+      'lid <- gensym ();
+      mret (val_of_ident (ID_Local lid), [I (IId lid) (INSTR_Op (SV (OP_ICmp cmp i64 v1 v2)))] ++ code2 ++ code1)
+  in
+  match b with
+  | BTrue => mret (val_of_bool true, [])
+  | BFalse => mret (val_of_bool false, [])
+  | BEq a1 a2 => compile_icmp Eq a1 a2
+  | BLe a1 a2 => compile_icmp Ule a1 a2
+  | BNot b =>
+    '(v, code) <- compile_bexp g b;
+    'lid <- gensym ();
+    mret (val_of_ident (ID_Local lid), [I (IId lid) (INSTR_Op (SV (OP_IBinop Xor i1 v (val_of_bool true))))] ++ code)
+  | BAnd b1 b2 =>
+    '(v1, code1) <- compile_bexp g b1;
+    '(v2, code2) <- compile_bexp g b2;
+    'lid <- gensym ();
+    mret (val_of_ident (ID_Local lid), [I (IId lid) (INSTR_Op (SV (OP_IBinop And i1 v1 v2)))] ++ code2 ++ code1)
+  end.
+
+Fixpoint compile_com (g:ctxt) (c:com) : GenSym (list elt) :=
+  match c with
+  | CSkip => mret []
+
+  | CAss x a =>
+    '(v, code) <- compile_aexp g a;
+    'uid <- lift (g x);
+    'vid <- genvoid ();
+    mret ((I vid (INSTR_Store false (i64, v) (i64ptr, val_of_ident uid) None)) :: code)
+
+  | CSeq c1 c2 =>
+    'code1 <- compile_com g c1;
+    'code2 <- compile_com g c2;
+    mret (code2 ++ code1)
+
+  | CIf b c1 c2 =>
+    '(v, codeb) <- compile_bexp g b;
+    'code1 <- compile_com g c1;
+    'code2 <- compile_com g c2;
+    'br1 <- gensym ();
+    'br2 <- gensym ();
+    'vid <- genvoid ();
+    mret (code2 ++ [L br2] ++ code1 ++ [L br1] ++ [T vid (TERM_Br (i1, v) br1 br2)] ++ codeb)
+
+  | CWhile b c =>
+    '(v, codeb) <- compile_bexp g b;
+    'code <- compile_com g c;
+    'entry <- gensym (); 
+    'body <- gensym (); 
+    'exit <- gensym ();
+    'vidbody <- genvoid ();
+    'videntry <- genvoid ();
+    'vidheader <- genvoid ();
+    mret ([L exit]
+            ++ [T vidbody (TERM_Br_1 entry)] ++ code ++ [L body]
+            ++ [T videntry (TERM_Br (i1, v) body exit)] ++ codeb ++ [L entry]
+            ++ [T vidheader (TERM_Br_1 entry)])
+  end.
+
+Fixpoint compile_fv (l:list id) : GenSym (ctxt * list elt) :=
+  match l with
+  | [] => mret (empty, [])
+  | x::xs =>
+    '(g, code) <- compile_fv xs;
+    'uid <- gensym ();
+    mret (update g x (ID_Local uid), [I (IId uid) (INSTR_Alloca i64 None None)]++code)  
+  end.
 
 
+Definition imp_prog_type := TYPE_Function TYPE_Void [].
+Definition imp_decl : declaration :=
+  {| dc_name := Name "imp_command";
+     dc_type := imp_prog_type;
+     dc_param_attrs := ([],[]);
+     dc_linkage := None;
+     dc_visibility := None;
+     dc_dll_storage := None;
+     dc_cconv := None;
+     dc_attrs := [];
+     dc_section := None;
+     dc_align := None;
+     dc_gc := None
+  |}.
 
 
-
-
+Definition compile (c:com) : option (definition (list block)) :=
+  'elts <-
+          run (
+            let fvs := fv c in
+            '(g, code_fv) <- compile_fv (IDSet.elements fvs);
+              'code <- compile_com g c;
+              mret (code ++ code_fv)
+          );
+  'blocks <- blocks_of_elts (Name "entry") elts;
+  mret {|
+    df_prototype := imp_decl;
+    df_args := [];
+    df_instrs := blocks
+  |}.
 
 
 
